Foundation/Propositional/Hilbert/VCorsi/Basic.lean
@@ -21,6 +21,7 @@ protected inductive Hilbert.VCorsi (Ax : Axiom α) : Logic α
 | protected andIR {φ ψ}             : Hilbert.VCorsi Ax φ → Hilbert.VCorsi Ax ψ → Hilbert.VCorsi Ax (φ ⋏ ψ)
 | protected dilemma {φ ψ χ}         : Hilbert.VCorsi Ax (φ ➝ χ) → Hilbert.VCorsi Ax (ψ ➝ χ) → Hilbert.VCorsi Ax (φ ⋎ ψ ➝ χ)
 | protected greedy {φ ψ χ}          : Hilbert.VCorsi Ax (φ ➝ ψ) → Hilbert.VCorsi Ax (φ ➝ χ) → Hilbert.VCorsi Ax (φ ➝ ψ ⋏ χ)
+| protected transRule {φ ψ χ}       : Hilbert.VCorsi Ax (φ ➝ ψ) → Hilbert.VCorsi Ax (ψ ➝ χ) → Hilbert.VCorsi Ax (φ ➝ χ)
 
 namespace Hilbert.VCorsi
 
@@ -58,19 +59,21 @@ instance : Entailment.VF (Hilbert.VCorsi Ax) where
   andIR! h₁ h₂ := ⟨VCorsi.andIR h₁.1 h₂.1⟩
   dilemma! h₁ h₂ := ⟨VCorsi.dilemma h₁.1 h₂.1⟩
   greedy! h₁ h₂ := ⟨VCorsi.greedy h₁.1 h₂.1⟩
+  transRule! h₁ h₂ := ⟨VCorsi.transRule h₁.1 h₂.1⟩
 
 @[induction_eliminator]
 protected lemma rec!
-  {motive   : (φ : Formula α) → (Hilbert.VCorsi Ax ⊢ φ) → Sort}
-  (axm      : ∀ {φ : Formula α} (s), (h : φ ∈ Ax) → motive (φ⟦s⟧) (VCorsi.axm! _ h))
-  (mdp      : ∀ {φ ψ : Formula α}, {hφψ : (Hilbert.VCorsi Ax) ⊢ φ ➝ ψ} → {hφ : (Hilbert.VCorsi Ax) ⊢ φ} → (motive (φ ➝ ψ) hφψ) → (motive φ hφ) → (motive ψ (hφψ ⨀ hφ)))
-  (af       : ∀ {φ ψ : Formula α}, {hφ : (Hilbert.VCorsi Ax) ⊢ φ} → (motive φ hφ) → (motive (ψ ➝ φ) (af hφ)))
-  (andIR    : ∀ {φ ψ : Formula α}, {hφ : (Hilbert.VCorsi Ax) ⊢ φ} → {hψ : (Hilbert.VCorsi Ax) ⊢ ψ} → (motive φ hφ) → (motive ψ hψ) → (motive (φ ⋏ ψ) (andIR hφ hψ)))
-  (dilemma  : ∀ {φ ψ χ : Formula α}, {h₁ : (Hilbert.VCorsi Ax) ⊢ φ ➝ χ} → {h₂ : (Hilbert.VCorsi Ax) ⊢ ψ ➝ χ} → (motive (φ ➝ χ) h₁) → (motive (ψ ➝ χ) h₂) → (motive (φ ⋎ ψ ➝ χ) (dilemma h₁ h₂)))
-  (greedy   : ∀ {φ ψ χ : Formula α}, {h₁ : (Hilbert.VCorsi Ax) ⊢ φ ➝ ψ} → {h₂ : (Hilbert.VCorsi Ax) ⊢ φ ➝ χ} → (motive (φ ➝ ψ) h₁) → (motive (φ ➝ χ) h₂) → (motive (φ ➝ ψ ⋏ χ) (greedy h₁ h₂)))
-  (impId    : ∀ {φ : Formula α}, (motive (Axioms.ImpId φ) impId))
-  (andElimL : ∀ {φ ψ : Formula α}, (motive (Axioms.AndElim₁ φ ψ) andElimL))
-  (andElimR : ∀ {φ ψ : Formula α}, (motive (Axioms.AndElim₂ φ ψ) andElimR))
+  {motive    : (φ : Formula α) → (Hilbert.VCorsi Ax ⊢ φ) → Sort}
+  (axm       : ∀ {φ : Formula α} (s), (h : φ ∈ Ax) → motive (φ⟦s⟧) (VCorsi.axm! _ h))
+  (mdp       : ∀ {φ ψ : Formula α}, {hφψ : (Hilbert.VCorsi Ax) ⊢ φ ➝ ψ} → {hφ : (Hilbert.VCorsi Ax) ⊢ φ} → (motive (φ ➝ ψ) hφψ) → (motive φ hφ) → (motive ψ (hφψ ⨀ hφ)))
+  (af        : ∀ {φ ψ : Formula α}, {hφ : (Hilbert.VCorsi Ax) ⊢ φ} → (motive φ hφ) → (motive (ψ ➝ φ) (af hφ)))
+  (andIR     : ∀ {φ ψ : Formula α}, {hφ : (Hilbert.VCorsi Ax) ⊢ φ} → {hψ : (Hilbert.VCorsi Ax) ⊢ ψ} → (motive φ hφ) → (motive ψ hψ) → (motive (φ ⋏ ψ) (andIR hφ hψ)))
+  (dilemma   : ∀ {φ ψ χ : Formula α}, {h₁ : (Hilbert.VCorsi Ax) ⊢ φ ➝ χ} → {h₂ : (Hilbert.VCorsi Ax) ⊢ ψ ➝ χ} → (motive (φ ➝ χ) h₁) → (motive (ψ ➝ χ) h₂) → (motive (φ ⋎ ψ ➝ χ) (dilemma h₁ h₂)))
+  (greedy    : ∀ {φ ψ χ : Formula α}, {h₁ : (Hilbert.VCorsi Ax) ⊢ φ ➝ ψ} → {h₂ : (Hilbert.VCorsi Ax) ⊢ φ ➝ χ} → (motive (φ ➝ ψ) h₁) → (motive (φ ➝ χ) h₂) → (motive (φ ➝ ψ ⋏ χ) (greedy h₁ h₂)))
+  (transRule : ∀ {φ ψ χ : Formula α}, {h₁ : (Hilbert.VCorsi Ax) ⊢ φ ➝ ψ} → {h₂ : (Hilbert.VCorsi Ax) ⊢ ψ ➝ χ} → (motive (φ ➝ ψ) h₁) → (motive (ψ ➝ χ) h₂) → (motive (φ ➝ χ) (transRule h₁ h₂)))
+  (impId     : ∀ {φ : Formula α}, (motive (Axioms.ImpId φ) impId))
+  (andElimL  : ∀ {φ ψ : Formula α}, (motive (Axioms.AndElim₁ φ ψ) andElimL))
+  (andElimR  : ∀ {φ ψ : Formula α}, (motive (Axioms.AndElim₂ φ ψ) andElimR))
   (orIntroL  : ∀ {φ ψ : Formula α}, (motive (Axioms.OrInst₁ φ ψ) orIntroL))
   (orIntroR  : ∀ {φ ψ : Formula α}, (motive (Axioms.OrInst₂ φ ψ) orIntroR))
   (distributeAndOr : ∀ {φ ψ χ : Formula α}, (motive (Axioms.DistributeAndOr φ ψ χ) distributeAndOr))
@@ -85,6 +88,7 @@ protected lemma rec!
   | andIR hφ hψ ihφ ihψ => apply andIR (ihφ (Logic.iff_provable.mpr hφ)) (ihψ (Logic.iff_provable.mpr hψ));
   | dilemma h₁ h₂ ih₁ ih₂ => apply dilemma (ih₁ (Logic.iff_provable.mpr h₁)) (ih₂ (Logic.iff_provable.mpr h₂));
   | greedy h₁ h₂ ih₁ ih₂ => apply greedy (ih₁ (Logic.iff_provable.mpr h₁)) (ih₂ (Logic.iff_provable.mpr h₂));
+  | transRule h₁ h₂ ih₁ ih₂ => apply transRule (ih₁ (Logic.iff_provable.mpr h₁)) (ih₂ (Logic.iff_provable.mpr h₂));
   | _ => grind;
 
 instance : Logic.Substitution (Hilbert.VCorsi Ax) where
@@ -96,6 +100,7 @@ instance : Logic.Substitution (Hilbert.VCorsi Ax) where
     | andIR ih₁ ih₂ => exact andIR ih₁ ih₂;
     | dilemma ih₁ ih₂ => exact dilemma ih₁ ih₂;
     | greedy ih₁ ih₂ => exact greedy ih₁ ih₂;
+    | transRule ih₁ ih₂ => exact transRule ih₁ ih₂;
     | _ =>
       first
       | apply impId;
@@ -116,6 +121,7 @@ lemma weakerThan_of_provable_axioms (hs : (Hilbert.VCorsi Ax₂) ⊢* Ax₁) : (
   | andIR ih₁ ih₂ => exact andIR ih₁ ih₂;
   | dilemma ih₁ ih₂ => exact dilemma ih₁ ih₂;
   | greedy ih₁ ih₂ => exact greedy ih₁ ih₂;
+  | transRule ih₁ ih₂ => exact transRule ih₁ ih₂;
   | _ =>
       first
       | apply impId;
