Foundation/Propositional/Entailment/Corsi.lean
@@ -1,3 +1,11 @@
 import Foundation.Propositional.Entailment.Corsi.Basic
 import Foundation.Propositional.Entailment.Corsi.F
 import Foundation.Propositional.Entailment.Corsi.VF
+
+namespace LO.Propositional.Entailment
+
+variable {S F : Type*} [DecidableEq F] [LogicalConnective F] [Entailment S F] {𝓢 : S}
+
+instance [Entailment.F 𝓢] : Entailment.VF 𝓢 where
+
+end LO.Propositional.Entailment
