Foundation/Propositional/FMT/Basic.lean
@@ -1,0 +1,312 @@
+/-
+  Fitting-Marek-Truszczyński Semantics
+-/
+import Foundation.Propositional.Logic.Basic
+import Foundation.Propositional.Entailment.Corsi.Basic
+import Foundation.Vorspiel.HRel.Basic
+
+namespace LO.Propositional
+
+namespace FMT
+
+structure Frame where
+  World : Type
+  Rel : Formula ℕ → HRel World
+  root : World
+  rooted {φ} {w : World} : Rel φ root w
+
+namespace Frame
+
+variable {F : Frame}
+
+attribute [simp, grind .] rooted
+
+instance : CoeSort Frame (Type) := ⟨World⟩
+instance : CoeFun Frame (λ F => Formula ℕ → HRel F.World) := ⟨Frame.Rel⟩
+instance : Nonempty F.World := ⟨F.root⟩
+
+abbrev Rel' {F : Frame} (φ : Formula ℕ) (x y : F.World) := F.Rel φ x y
+notation:45 x:90 " ≺[" φ "] " y:90 => Frame.Rel' φ x y
+
+
+notation:45 x:max " ≺[" φ "] " y:max " on " F:max => Frame.Rel F φ x y
+
+end Frame
+
+abbrev FrameClass := Set Frame
+
+
+
+abbrev Valuation (F : Frame) := F.World → ℕ → Prop
+
+
+structure Model extends Frame where
+  Val : Valuation toFrame
+
+namespace Model
+
+instance : CoeSort (Model) (Type) := ⟨λ M => M.World⟩
+instance : CoeFun (Model) (λ M => M.World → ℕ → Prop) := ⟨fun m => m.Val⟩
+
+end Model
+
+abbrev ModelClass := Set Model
+
+end FMT
+
+
+
+namespace Formula.FMT
+
+open FMT
+
+def Satisfies (M : FMT.Model) (x : M.World) : Formula ℕ → Prop
+  | atom a => M x a
+  | ⊥      => False
+  | φ ⋏ ψ  => Satisfies M x φ ∧ Satisfies M x ψ
+  | φ ⋎ ψ  => Satisfies M x φ ∨ Satisfies M x ψ
+  | φ ➝ ψ => ∀ {y : M.World}, x ≺[φ] y → (Satisfies M y φ → Satisfies M y ψ)
+
+namespace Satisfies
+
+instance semantics (M : FMT.Model) : Semantics M (Formula ℕ) := ⟨fun x ↦ Formula.FMT.Satisfies M x⟩
+
+variable {M : FMT.Model} {x y : M.World} {a : ℕ} {φ ψ χ : Formula ℕ}
+
+@[simp, grind =] protected lemma iff_models : x ⊧ φ ↔ Satisfies M x φ := iff_of_eq rfl
+
+@[grind =] protected lemma def_atom : x ⊧ atom a ↔ M x a := by simp [Satisfies];
+@[simp high, grind .] protected lemma def_top : x ⊧ ⊤ := by simp [Satisfies];
+@[simp high, grind .] protected lemma def_bot : x ⊭ ⊥ := by simp [Semantics.NotModels, Satisfies];
+
+@[grind =] protected lemma def_and : x ⊧ φ ⋏ ψ ↔ x ⊧ φ ∧ x ⊧ ψ := by simp [Satisfies];
+@[grind =] protected lemma not_def_and : x ⊭ φ ⋏ ψ ↔ x ⊭ φ ∨ x ⊭ ψ := by
+  dsimp [Semantics.NotModels];
+  grind;
+
+@[grind =] protected lemma def_or  : x ⊧ φ ⋎ ψ ↔ x ⊧ φ ∨ x ⊧ ψ := by simp [Satisfies];
+@[grind =] protected lemma not_def_or : x ⊭ φ ⋎ ψ ↔ x ⊭ φ ∧ x ⊭ ψ := by
+  dsimp [Semantics.NotModels];
+  grind;
+
+@[grind =] protected lemma def_imp  : x ⊧ φ ➝ ψ ↔ ∀ {y : M.World}, (x ≺[φ] y) → (y ⊧ φ → y ⊧ ψ) := by simp [Satisfies];
+@[grind =] protected lemma not_def_imp : x ⊭ φ ➝ ψ ↔ ∃ y : M.World, (x ≺[φ] y) ∧ (y ⊧ φ) ∧ (y ⊭ ψ) := by
+  dsimp [Semantics.NotModels];
+  grind;
+
+@[grind =] protected lemma def_neg  : x ⊧ ∼φ ↔ ∀ {y : M.World}, (x ≺[φ] y) → ¬(y ⊧ φ) := by simp [Satisfies];
+@[grind =] protected lemma not_def_neg : x ⊭ ∼φ ↔ ∃ y : M.World, (x ≺[φ] y) ∧ (y ⊧ φ) := by grind;
+
+instance : Semantics.Top M.World := ⟨by grind⟩
+instance : Semantics.Bot M.World := ⟨by grind⟩
+instance : Semantics.And M.World := ⟨by grind⟩
+instance : Semantics.Or M.World := ⟨by grind⟩
+
+/-
+lemma iff_subst_self {F : FMT.Frame} {V : FMT.Valuation F} {x : F.World} (s : Substitution ℕ) :
+  letI U : FMT.Valuation F := λ w a => Satisfies ⟨F, V⟩ w ((.atom a)⟦s⟧)
+  Satisfies ⟨F, U⟩ x φ ↔ Satisfies ⟨F, V⟩ x (φ⟦s⟧) := by
+  induction φ generalizing x with
+  | hatom a => simp [Satisfies];
+  | hfalsum => simp [Satisfies];
+  | hand φ ψ ihφ ihψ =>
+    constructor;
+    . rintro ⟨hφ, hψ⟩; constructor <;> grind
+    . rintro ⟨hφ, hψ⟩; constructor <;> grind;
+  | hor φ ψ ihφ ihψ =>
+    constructor;
+    . rintro (hφ | hψ);
+      . left; apply ihφ.mp hφ;
+      . right; apply ihψ.mp hψ;
+    . rintro (hφ | hψ);
+      . left; apply ihφ.mpr hφ;
+      . right; apply ihψ.mpr hψ;
+  | himp φ ψ ihφ ihψ =>
+    constructor;
+    . intro hφψ y Rxy hφs;
+      apply ihψ.mp;
+      apply hφψ;
+      apply hφψ Rxy;
+      apply ihφ.mpr hφs;
+    . intro hφψs y Rxy hφ;
+      apply ihψ.mpr;
+      apply hφψs Rxy;
+      apply ihφ.mp hφ;
+-/
+
+end Satisfies
+
+
+def ValidOnModel (M : FMT.Model) (φ : Formula ℕ) : Prop := ∀ x : M.World, Satisfies M x φ
+
+namespace ValidOnModel
+
+instance semantics : Semantics FMT.Model (Formula ℕ) := ⟨fun M ↦ ValidOnModel M⟩
+
+variable {M : FMT.Model} {φ ψ χ : Formula ℕ}
+
+@[simp, grind =] protected lemma iff_models : M ⊧ φ ↔ ∀ x : M, x ⊧ φ := iff_of_eq rfl
+
+@[grind .] protected lemma def_verum : M ⊧ ⊤ := by simp;
+@[grind .] protected lemma def_bot : M ⊭ ⊥ := by simp [Semantics.NotModels];
+
+instance : Semantics.Top (FMT.Model) := ⟨by grind⟩
+instance : Semantics.Bot (FMT.Model) := ⟨by grind⟩
+
+lemma iff_not_models_exists_world : (M ⊭ φ) ↔ (∃ x : M.World, ¬x ⊧ φ) := by grind;
+alias ⟨exists_world_of_not, not_of_exists_world⟩ := iff_not_models_exists_world
+
+
+end ValidOnModel
+
+
+def ValidOnFrame (F : FMT.Frame) (φ : Formula ℕ) : Prop := ∀ V : FMT.Valuation F, (⟨F, V⟩ : FMT.Model) ⊧ φ
+
+namespace ValidOnFrame
+
+instance semantics : Semantics FMT.Frame (Formula ℕ) := ⟨fun F ↦ ValidOnFrame F⟩
+
+variable {F : FMT.Frame} {φ ψ χ : Formula ℕ}
+
+@[simp, grind =] protected lemma iff_models : F ⊧ φ ↔ ∀ V : FMT.Valuation F, (⟨F, V⟩ : FMT.Model) ⊧ φ := iff_of_eq rfl
+
+@[grind .] protected lemma def_verum : F ⊧ ⊤ := by simp;
+@[grind .] protected lemma def_bot : F ⊭ ⊥ := by simp [Semantics.NotModels];
+
+instance : Semantics.Top (FMT.Frame) := ⟨by grind⟩
+instance : Semantics.Bot (FMT.Frame) := ⟨by grind⟩
+
+
+lemma iff_not_exists_valuation : (F ⊭ φ) ↔ (∃ V : FMT.Valuation F, ¬(⟨F, V⟩ : FMT.Model) ⊧ φ) := by grind;
+alias ⟨exists_valuation_of_not, not_of_exists_valuation⟩ := iff_not_exists_valuation
+
+
+lemma iff_not_exists_valuation_world : (F ⊭ φ) ↔ (∃ V : FMT.Valuation F, ∃ x : (⟨F, V⟩ : FMT.Model).World, ¬Satisfies _ x φ) := by
+  simp [ValidOnFrame, ValidOnModel, Semantics.Models, Semantics.NotModels];
+alias ⟨exists_valuation_world_of_not, not_of_exists_valuation_world⟩ := iff_not_exists_valuation_world
+
+/-
+@[grind =>]
+protected lemma subst (s : Substitution ℕ) (h : F ⊧ φ) : F ⊧ φ⟦s⟧ := by
+  by_contra hC;
+  obtain ⟨V, ⟨x, hx⟩⟩ := exists_valuation_world_of_not hC;
+  apply Satisfies.iff_subst_self s |>.not.mpr hx;
+  apply h;
+-/
+
+end ValidOnFrame
+
+end Formula.FMT
+
+
+namespace FMT
+
+
+open Formula.FMT
+
+
+section
+
+variable {C : Set Frame} {φ ψ χ : Formula ℕ}
+
+lemma iff_not_validOnFrameClass_exists_frame : C ⊭ φ ↔ ∃ F ∈ C, ¬F ⊧ φ := by
+  apply not_iff_not.mp;
+  push_neg;
+  tauto;
+alias ⟨exists_frame_of_not_validOnFrameClass, not_validOnFrameClass_of_exists_frame⟩ := iff_not_validOnFrameClass_exists_frame
+
+lemma iff_not_validOnFrameClass_exists_model : C ⊭ φ ↔ ∃ M : FMT.Model, M.toFrame ∈ C ∧ M ⊭ φ := by
+  apply not_iff_not.mp;
+  push_neg;
+  tauto;
+alias ⟨exists_model_of_not_validOnFrameClass, not_validOnFrameClass_of_exists_model⟩ := iff_not_validOnFrameClass_exists_model
+
+lemma iff_not_validOnFrameClass_exists_model_world : C ⊭ φ ↔ ∃ M : FMT.Model, ∃ x : M, M.toFrame ∈ C ∧ x ⊭ φ := by
+  apply not_iff_not.mp;
+  push_neg;
+  tauto;
+alias ⟨exists_model_world_of_not_validOnFrameClass, not_validOnFrameClass_of_exists_model_world⟩ := iff_not_validOnFrameClass_exists_model_world
+
+end
+
+
+section
+
+variable {F : Frame} {φ ψ χ : Formula ℕ}
+
+open Formula (atom)
+
+lemma valid_andElim₁ : F ⊧ Axioms.AndElim₁ φ ψ := by rintro V x y Rxy ⟨_, _⟩; assumption;
+lemma valid_andElim₂ : F ⊧ Axioms.AndElim₂ φ ψ := by rintro V x y Rxy ⟨_, _⟩; assumption;
+lemma valid_axiomC : F ⊧ Axioms.C φ ψ χ := by
+  rintro V x y Rxy ⟨h₁, h₂⟩ z Ryz h₃;
+  constructor;
+  . apply h₁ <;> assumption;
+  . apply h₂;
+    . assumption;
+    . assumption;
+
+lemma valid_orIntro₁ : F ⊧ Axioms.OrInst₁ φ ψ := by rintro V x y Rxy hφ; left; assumption;
+lemma valid_orIntro₂ : F ⊧ Axioms.OrInst₂ φ ψ := by rintro V x y Rxy hψ; right; assumption;
+
+lemma valid_distributeAndOr : F ⊧ Axioms.DistributeAndOr φ ψ χ := by
+  rintro V x y Rxy ⟨hφ, (hψ | hχ)⟩
+  . left; constructor <;> assumption;
+  . right; constructor <;> assumption;
+lemma valid_impId : F ⊧ Axioms.ImpId φ := by rintro V x y Rxy hφ; assumption;
+
+attribute [simp high, grind .]
+  valid_andElim₁ valid_andElim₂
+  valid_axiomC
+  valid_orIntro₁ valid_orIntro₂
+  valid_distributeAndOr
+  valid_impId
+
+@[grind <=]
+lemma valid_afortiori (h : F ⊧ φ) : F ⊧ ψ ➝ φ := by
+  rintro V x y Rxy _;
+  apply h;
+
+@[grind <=]
+lemma valid_conjunction_rule (h₁ : F ⊧ φ) (h₂ : F ⊧ ψ) : F ⊧ φ ⋏ ψ := by
+  rintro V x;
+  constructor;
+  . apply h₁;
+  . apply h₂;
+
+@[grind ⇒]
+lemma valid_modusponens (h₁ : F ⊧ φ ➝ ψ) (h₂ : F ⊧ φ) : F ⊧ ψ := by
+  rintro V x;
+  apply h₁;
+  . apply F.rooted;
+  . apply h₂;
+
+@[grind <=]
+lemma valid_dilemma (h₁ : F ⊧ φ ➝ χ) (h₂ : F ⊧ ψ ➝ χ) : F ⊧ φ ⋎ ψ ➝ χ := by
+  rintro V x y Rxy (hφ | hψ);
+  . apply h₁ _ F.root <;> grind;
+  . apply h₂ _ F.root <;> grind;
+
+@[grind <=]
+lemma valid_greedy (h₁ : F ⊧ φ ➝ ψ) (h₂ : F ⊧ φ ➝ χ) : F ⊧ φ ➝ ψ ⋏ χ := by
+  rintro V x y Rxy hφ;
+  constructor;
+  . apply h₁ _ x <;> grind;
+  . apply h₂ _ x <;> grind;
+
+@[grind <=]
+lemma valid_CTrans (h₁ : F ⊧ φ ➝ ψ) (h₂ : F ⊧ ψ ➝ χ) : F ⊧ φ ➝ χ := by
+  intro V x y Rxy hyφ;
+  apply h₂ _ F.root;
+  . apply F.rooted;
+  . apply h₁ _ F.root;
+    . apply F.rooted;
+    . assumption;
+
+
+end
+
+end FMT
+
+
+end LO.Propositional
