Foundation/Propositional/FMT/Logic/VF.lean
@@ -1,0 +1,118 @@
+import Foundation.Propositional.FMT.Hilbert
+import Foundation.Propositional.Hilbert.VCorsi.Disjunctive
+import Foundation.Propositional.Hilbert.Corsi.Basic
+import Foundation.Propositional.Hilbert.Corsi_VCorsi
+
+namespace LO.Propositional
+
+open FMT
+
+
+namespace FMT
+
+protected abbrev FrameClass.VF : FMT.FrameClass := Set.univ
+
+abbrev trivialFrame : FMT.Frame where
+  World := Unit
+  Rel _ _ _ := True
+  root := ()
+  rooted := by simp
+
+end FMT
+
+
+namespace VF
+
+open Hilbert.VCorsi.FMT
+
+instance FMT.sound : Sound Propositional.VF FrameClass.VF := by
+  apply instFrameClassSound;
+  constructor;
+  simp;
+
+instance : Entailment.Consistent Propositional.VF := consistent_of_sound_frameclass FrameClass.VF $ by
+  use FMT.trivialFrame;
+  apply Set.mem_setOf_eq.mpr;
+  simp;
+
+open Formula.FMT in
+lemma unprovable_axiomD : Propositional.VF ⊬ Axioms.D #0 #1 #2 := by
+  apply Sound.not_provable_of_countermodel (𝓜 := FrameClass.VF);
+  apply FMT.not_validOnFrameClass_of_exists_frame;
+  use {
+    World := Fin 3,
+    Rel := λ φ x y =>
+      match φ, x, y with
+      | _, 0, _ => True
+      | φ, 1, 2 => φ = #0 ⋎ #1
+      | _, _, _ => False
+    ,
+    root := 0,
+    rooted := by tauto
+  };
+  constructor;
+  . tauto;
+  . apply ValidOnFrame.not_of_exists_valuation_world;
+    use λ w a => match w, a with
+      | 2, 2 => False
+      | _, _ => True;
+    use 0;
+    apply Satisfies.not_def_imp.mpr;
+    use 1;
+    constructor;
+    . tauto;
+    . constructor;
+      . constructor;
+        . intro z; match z with | 0 | 1 | 2 => tauto
+        . intro z; match z with | 0 | 1 | 2 => tauto
+      . apply Satisfies.not_def_imp.mpr;
+        use 2;
+        tauto;
+
+open Formula.FMT in
+lemma unprovable_axiomI : Propositional.VF ⊬ Axioms.I #0 #1 #2 := by
+  apply Sound.not_provable_of_countermodel (𝓜 := FrameClass.VF);
+  apply FMT.not_validOnFrameClass_of_exists_frame;
+  use {
+    World := Fin 3,
+    Rel := λ φ x y =>
+      match φ, x, y with
+      | _, 0, _ => True
+      | φ, 1, 2 => φ = #0
+      | _, _, _ => False
+    ,
+    root := 0,
+    rooted := by tauto
+  };
+  constructor;
+  . tauto;
+  . apply ValidOnFrame.not_of_exists_valuation_world;
+    use λ w a => match w, a with
+      | 2, 2 => False
+      | _, _ => True;
+    use 0;
+    apply Satisfies.not_def_imp.mpr;
+    use 1;
+    refine ⟨?_, ?_, ?_⟩;
+    . tauto;
+    . constructor;
+      . simp [Satisfies]
+      . intro z R1z; match z with | 0 | 1 | 2 => grind;
+    . apply Satisfies.not_def_imp.mpr;
+      use 2;
+      tauto;
+
+end VF
+
+instance : Propositional.VF ⪱ Propositional.F := by
+  constructor;
+  . apply weakerThan_VCorsi_Corsi_of_provable_axiomInstances;
+    intro φ;
+    simp;
+  . apply Entailment.not_weakerThan_iff.mpr;
+    use (Axioms.D #0 #1 #2);
+    constructor;
+    . simp;
+    . exact VF.unprovable_axiomD
+
+end LO.Propositional
