Foundation/Propositional/Hilbert/Corsi_VCorsi.lean
@@ -1,0 +1,25 @@
+import Foundation.Propositional.Hilbert.Corsi.Basic
+import Foundation.Propositional.Hilbert.VCorsi.Basic
+
+namespace LO.Propositional
+
+open Entailment.Corsi
+
+def weakerThan_VCorsi_Corsi_of_provable_axiomInstances (h : (Hilbert.Corsi Ax₂) ⊢* Ax₁.instances) : (Hilbert.VCorsi Ax₁) ⪯ (Hilbert.Corsi Ax₂) := by
+  apply Logic.weakerThan_of_provable;
+  intro φ hφ;
+  induction hφ using Hilbert.VCorsi.rec! with
+  | axm => apply h; grind;
+  | mdp ihφψ ihφ => exact ihφψ ⨀ ihφ;
+  | _ =>
+    first
+    | apply impId;
+    | apply andElimL;
+    | apply andElimR;
+    | apply orIntroL;
+    | apply orIntroR;
+    | apply distributeAndOr;
+    | apply axiomC;
+    | grind;
+
+end LO.Propositional
